src/example/SCM.v
@@ -148,7 +148,7 @@ Module SCMem.
     end.
 
   Definition alloc_fun:
-    ktree (((@eventE ident) +' cE) +' sE t) nat val :=
+    ktree (programE ident t) nat val :=
     fun sz =>
       m <- trigger (@Get _);;
       let (m, v) := alloc m sz in
@@ -157,7 +157,7 @@ Module SCMem.
   .
 
   Definition store_fun:
-    ktree (((@eventE ident) +' cE) +' sE t) (val * val) unit :=
+    ktree (programE ident t) (val * val) unit :=
     fun '(vptr, v) =>
       m <- trigger (@Get _);;
       m <- unwrap (store m vptr v);;
@@ -166,7 +166,7 @@ Module SCMem.
   .
 
   Definition load_fun:
-    ktree (((@eventE ident) +' cE) +' sE t) val val :=
+    ktree (programE ident t) val val :=
     fun vptr =>
       m <- trigger (@Get _);;
       v <- unwrap (load m vptr);;
@@ -174,7 +174,7 @@ Module SCMem.
   .
 
   Definition faa_fun:
-    ktree (((@eventE ident) +' cE) +' sE t) (val * nat) val :=
+    ktree (programE ident  t) (val * nat) val :=
     fun '(vptr, addend) =>
       m <- trigger (@Get _);;
       '(m, v) <- unwrap (faa m vptr addend);;
@@ -183,7 +183,7 @@ Module SCMem.
   .
 
   Definition cas_fun:
-    ktree (((@eventE ident) +' cE) +' sE t) (val * val * val) bool :=
+    ktree (programE ident t) (val * val * val) bool :=
     fun '(vptr, v_old, v_new) =>
       m <- trigger (@Get _);;
       mb <- unwrap (cas m vptr v_old v_new);;
@@ -197,7 +197,7 @@ Module SCMem.
   .
 
   Definition cas_weak_fun:
-    ktree (((@eventE ident) +' cE) +' sE t) (val * val * val) bool :=
+    ktree (programE ident t) (val * val * val) bool :=
     fun '(vptr, v_old, v_new) =>
       m <- trigger (@Get _);;
       b <- trigger (Choose bool);;
@@ -220,7 +220,7 @@ Module SCMem.
   .
 
   Definition compare_fun:
-    ktree (((@eventE ident) +' cE) +' sE t) (val * val) bool :=
+    ktree (programE ident t) (val * val) bool :=
     fun '(v0, v1) =>
       m <- trigger (@Get _);;
       b <- unwrap (compare m v0 v1);;
