src/example/WMM.v
@@ -33,7 +33,7 @@ Module WMem.
       else Flag.emp.
 
   Definition load_fun:
-    ktree (((@eventE ident) +' cE) +' sE t) (TView.t * Loc.t * Ordering.t) (TView.t * Const.t) :=
+    ktree (programE ident t) (TView.t * Loc.t * Ordering.t) (TView.t * Const.t) :=
     fun '(tvw0, loc, ord) =>
       msc <- trigger (@Get _);;
       '(exist _ (lc1, val, to) _) <- trigger (Choose (sig (fun '(lc1, val, to) =>
@@ -52,7 +52,7 @@ Module WMem.
   .
 
   Definition store_fun:
-    ktree (((@eventE ident) +' cE) +' sE t) (TView.t * Loc.t * Const.t * Ordering.t) (TView.t) :=
+    ktree (programE ident t) (TView.t * Loc.t * Const.t * Ordering.t) (TView.t) :=
     fun '(tvw0, loc, val, ord) =>
       msc <- trigger (@Get _);;
       '(exist _ (lc1, to, sc1, mem1) _) <- trigger (Choose (sig (fun '(lc1, to, sc1, mem1) =>
@@ -78,7 +78,7 @@ Module WMem.
   .
 
   Definition faa_fun:
-    ktree (((@eventE ident) +' cE) +' sE t) (TView.t * Loc.t * Const.t * Ordering.t * Ordering.t) (TView.t * Const.t) :=
+    ktree (programE ident t) (TView.t * Loc.t * Const.t * Ordering.t * Ordering.t) (TView.t * Const.t) :=
     fun '(tvw0, loc, addendum, ordr, ordw) =>
       msc <- trigger (@Get _);;
       '(exist _ (lc1, to, val, sc1, mem1) _) <- trigger (Choose (sig (fun '(lc2, from, val, sc1, mem1) =>
