src/simulation/ModCloseSim.v
@@ -41,7 +41,7 @@ Section CLOSE_CONG_SIM.
   Opaque lifted threadsRA URA.prod.
 
   Lemma lift_ma_local_sim_ub R_src R_tgt (RR : R_src -> R_tgt -> Prop) ktr_src itr_tgt
-    : local_sim lift_ma RR (Vis (inl1 (inl1 Undefined)) ktr_src) itr_tgt.
+    : local_sim lift_ma RR (Vis (inl1 (inl1 (inl1 Undefined))) ktr_src) itr_tgt.
   Proof.
     (* treat as if tid ∈ ths_ctx *)
     intros ths IM_SRC0 IM_TGT0 st_src0 st_tgt0 [r_sha_th0 r_sha_w0] [r_ctx_th0 r_ctx_w0] INV0_0 tid ths0 THS0 VALID0_0 IM_TGT1 TID_TGT.
