src/simulation/ModSimYOrd.v
@@ -25,8 +25,8 @@ Section PRIMIVIESIM.
   Variable wf_src: WF.
   Variable wf_tgt: WF.
 
-  Let srcE := ((@eventE ident_src +' cE) +' sE state_src).
-  Let tgtE := ((@eventE _ident_tgt +' cE) +' sE state_tgt).
+  Let srcE := programE ident_src state_src.
+  Let tgtE := programE _ident_tgt state_tgt.
 
   Definition shared :=
     (TIdSet.t *
