src/simulation/Stutter2Knot.v
@@ -31,8 +31,8 @@ Section PROOF.
   Variable wf_src: WF.
   Variable wf_tgt: WF.
 
-  Notation srcE := ((@eventE _ident_src +' cE) +' sE state_src).
-  Notation tgtE := ((@eventE _ident_tgt +' cE) +' sE state_tgt).
+  Notation srcE := (programE _ident_src state_src).
+  Notation tgtE := (programE _ident_tgt state_tgt).
 
   Variable wf_stt: Type -> Type -> WF.
 
